getting closer

LeanSAT/Reflect/BoolExpr/Tseitin.lean
@@ -21,6 +21,9 @@ import Std.Tactic.LibrarySearch
 theorem eq_true_or_eq_false {x : Bool} : x = true ∨ x = false := by cases x <;> simp
 theorem eq_false_or_eq_true {x : Bool} : x = false ∨ x = true := by cases x <;> simp
 
+@[simp] theorem Bool.eq_not {x : Bool} : x = (!x) ↔ False := by cases x <;> simp
+@[simp] theorem Bool.not_eq {x : Bool} : (!x) = x ↔ False := by cases x <;> simp
+
 namespace Gate
 
 def toCNF (i₁ i₂ o : α) : Gate → CNF α
@@ -116,6 +119,14 @@ where
       | (cy, ny) =>
         (g.toCNF (.inr nx) (.inr ny) (.inr (ny + 1)) ++ cx ++ cy, ny + 1)
 
+def toCNF'_relabel (k : Nat) : α ⊕ Nat → α ⊕ Nat
+  | .inl a => .inl a
+  | .inr i => .inr (k + i)
+
+theorem toCNF'.run_fst_eq_relabel (k) (x : BoolExpr α) :
+    (toCNF'.run k x).1 = (toCNF'.run 0 x).1.relabel (toCNF'_relabel k) :=
+  sorry
+
 @[simp] theorem toCNF'_run_snd (x : BoolExpr α) : (toCNF'.run k x).2 = k + x.size - 1 := by
   match x with
   | .literal _
@@ -124,6 +135,45 @@ where
   | .gate _ x y =>
     have := x.size_pos
     simp [toCNF'.run, size, toCNF'_run_snd] <;> omega
+
+theorem bounds_of_inr_mem_toCNF'_run_fst {i : Nat} {x : BoolExpr α}
+    (w : .inr i ∈ (toCNF'.run k x).1) : k ≤ i ∧ i < k + x.size := by
+  match x with
+  | .literal a =>
+    simp [toCNF'.run, size, CNF.eq] at *
+    omega
+  | .const b =>
+    simp [toCNF'.run, size] at *
+    omega
+  | .not x =>
+    have := x.size_pos
+    simp [toCNF'.run, size, CNF.ne] at *
+    cases w
+    case inl h => omega
+    case inr h =>
+      replace h := bounds_of_inr_mem_toCNF'_run_fst h
+      omega
+  | .gate g x y =>
+    have := x.size_pos
+    have := y.size_pos
+    simp [toCNF'.run, size, CNF.ne] at *
+    rcases w with (w | w | w)
+    · cases g
+      all_goals
+        simp [Gate.toCNF] at w
+        omega
+    · replace w := bounds_of_inr_mem_toCNF'_run_fst w
+      omega
+    · replace w := bounds_of_inr_mem_toCNF'_run_fst w
+      omega
+
+theorem ge_of_inr_mem_toCNF'_run_fst {i : Nat} {x : BoolExpr α}
+    (w : .inr i ∈ (toCNF'.run k x).1) : k ≤ i :=
+  (bounds_of_inr_mem_toCNF'_run_fst w).1
+
+theorem lt_of_inr_mem_toCNF'_run_fst {i : Nat} {x : BoolExpr α}
+    (w : .inr i ∈ (toCNF'.run k x).1) : i < k + x.size :=
+  (bounds_of_inr_mem_toCNF'_run_fst w).2
 
 theorem toCNF'_run_eval (k : Nat) (x : BoolExpr α) (f : α ⊕ Nat → Bool) :
     let (c, p) := toCNF'.run k x
@@ -169,7 +219,10 @@ theorem toCNF'_eval (x : BoolExpr α) (f : α ⊕ Nat → Bool) :
   cases x1 <;> cases x2 <;> simp
 
 -- the output of the `k`-th gate
-def traceEval (x : BoolExpr α) (f : α → Bool) (l : Nat) : Bool :=
+-- This definition is marked noncomputable to mark sure no one accidentally tries to run it.
+-- It is very inefficient (traversing the `BoolExpr` for each evaluation)
+-- and only intended as an auxiliary construction for the proofs!
+noncomputable def traceEval (x : BoolExpr α) (f : α → Bool) (l : Nat) : Bool :=
   (run 0 x).1
 where
   run (k : Nat) : BoolExpr α → Bool × Bool × Nat
@@ -182,7 +235,27 @@ where
       | (ry, dy, ky) =>
         (bif dx then rx else bif dy then ry else g.eval rx ry, dx || dy || (ky + 1 = l), ky + 1)
 
-theorem traceEval_run_snd_snd : (traceEval.run f l k x).2.2 = k + x.size - 1 := by
+theorem traceEval_run_eq : (match (traceEval.run f i 0 x) with | ⟨r, d, c⟩ => ⟨r, d, c + k⟩) =
+    traceEval.run f (k + i) k x := by
+  match x with
+  | .literal a => simp [traceEval.run]; omega
+  | .const b => simp [traceEval.run]; omega
+  | .not x => simp [traceEval.run, ← traceEval_run_eq]; sorry
+  | .gate g x y => sorry
+
+theorem traceEval_run_fst_eq : (traceEval.run f i 0 x).fst = (traceEval.run f (k + i) k x).fst := by
+  sorry
+
+theorem elim_traceEval_eq_comp (k) :
+    Sum.elim f (traceEval x f) =
+      (Sum.elim f fun l => (traceEval.run f l k x).1) ∘ (toCNF'_relabel k) := by
+  funext i
+  rcases i with (a | i)
+  · simp [toCNF'_relabel]
+  · simp [toCNF'_relabel, traceEval]
+    apply traceEval_run_fst_eq
+
+@[simp] theorem traceEval_run_snd_snd : (traceEval.run f l k x).2.2 = k + x.size - 1 := by
   match x with
   | .literal _ => simp [size, traceEval.run]
   | .const _ => simp [size, traceEval.run]
@@ -197,7 +270,7 @@ theorem traceEval_run_snd_snd : (traceEval.run f l k x).2.2 = k + x.size - 1 := 
     rw [traceEval_run_snd_snd, traceEval_run_snd_snd]
     omega
 
-theorem traceEval_run_snd_fst_of_le (w : k + x.size ≤ l) : (traceEval.run f l k x).2.1 = false := by
+theorem traceEval_run_snd_fst_of_le (x) (w : k + x.size ≤ l) : (traceEval.run f l k x).2.1 = false := by
   match x with
   | .literal a => simp [size, traceEval.run] at *; omega
   | .const b => simp [size, traceEval.run] at *; omega
@@ -217,7 +290,7 @@ theorem traceEval_run_snd_fst_of_le (w : k + x.size ≤ l) : (traceEval.run f l 
     simp only [Bool.or_self, Bool.false_or, decide_eq_false_iff_not, ne_eq]
     all_goals omega
 
-theorem traceEval_run_snd_fst (w₁ : k ≤ l) (w₂ : l < k + x.size) : (traceEval.run f l k x).2.1 = true := by
+theorem traceEval_run_snd_fst (x) (w₁ : k ≤ l) (w₂ : l < k + x.size) : (traceEval.run f l k x).2.1 = true := by
   match x with
   | .literal a => simp [size, traceEval.run] at *; omega
   | .const b => simp [size, traceEval.run] at *; omega
@@ -266,10 +339,182 @@ theorem traceEval_run_fst (w : k + x.size - 1 ≤ l) : (traceEval.run f l k x).1
     have := x.size_pos
     have := y.size_pos
     simp [size, traceEval.run] at *
-    rw [traceEval_run_snd_snd, traceEval_run_snd_fst_of_le, traceEval_run_snd_fst_of_le,
+    rw [traceEval_run_snd_fst_of_le, traceEval_run_snd_fst_of_le,
       traceEval_run_fst, traceEval_run_fst]
     simp only [cond_false]
     all_goals omega
+
+@[simp] theorem traceEval_size_sub_one : traceEval x f (size x - 1) = x.eval f := by
+  dsimp [traceEval]
+  rw [traceEval_run_fst]
+  omega
+
+theorem traceEval_not (w : l < x.size) : traceEval (not x) f l = traceEval x f l := by
+  match x with
+  | .literal a =>
+    simp [traceEval, traceEval.run, size] at *
+    rw [cond_eq_if, if_pos]; simp; omega
+  | .const b =>
+    simp [traceEval, traceEval.run, size] at *
+    rw [cond_eq_if, if_pos]; simp; omega
+  | .not x =>
+    have := x.size_pos
+    simp [traceEval, traceEval.run, size] at *
+    if h : l < x.size then
+      rw [traceEval_run_snd_fst]
+      simp
+      all_goals omega
+    else
+      rw [traceEval_run_snd_fst_of_le]
+      simp [cond_eq_if]
+      all_goals omega
+  | .gate g x y =>
+    have := x.size_pos
+    have := y.size_pos
+    simp [traceEval, traceEval.run, size] at *
+    if h : l < x.size then
+      rw [traceEval_run_snd_fst x]
+      simp
+      all_goals omega
+    else
+      if h : l < x.size + y.size then
+        rw [traceEval_run_snd_fst y]
+        simp
+        all_goals omega
+      else
+        rw [traceEval_run_snd_fst_of_le x]
+        rw [traceEval_run_snd_fst_of_le y]
+        simp [cond_eq_if]
+        all_goals omega
+
+theorem traceEval_gate_left (w : l < x.size) : traceEval (gate g x z) f l = traceEval x f l := by
+  match x with
+  | .literal a =>
+    simp [traceEval, traceEval.run, size] at *
+    rw [cond_eq_if, if_pos]; simp; omega
+  | .const b =>
+    simp [traceEval, traceEval.run, size] at *
+    rw [cond_eq_if, if_pos]; simp; omega
+  | .not x =>
+    have := x.size_pos
+    simp [traceEval, traceEval.run, size] at *
+    if h : l < x.size then
+      rw [traceEval_run_snd_fst x (by omega) (by omega)]
+      simp
+    else
+      rw [traceEval_run_snd_fst_of_le x (by omega)]
+      simp [cond_eq_if]
+      omega
+  | .gate g x y =>
+    have := x.size_pos
+    have := y.size_pos
+    simp [traceEval, traceEval.run, size] at *
+    if h : l < x.size then
+      rw [traceEval_run_snd_fst x (by omega) (by omega)]
+      simp
+    else
+      if h : l < x.size + y.size then
+        rw [traceEval_run_snd_fst y (by omega) (by omega)]
+        simp
+      else
+        rw [traceEval_run_snd_fst_of_le x (by omega)]
+        rw [traceEval_run_snd_fst_of_le y (by omega)]
+        simp [cond_eq_if]
+        omega
+
+theorem traceEval_gate_right (w₁ : x.size ≤ l) (w₂ : l < x.size + y.size) :
+    traceEval (gate g x y) f l = (traceEval.run f l x.size y).1 := by
+  have := x.size_pos
+  match y with
+  | .literal a =>
+    simp [traceEval, traceEval.run, size] at *
+    rw [traceEval_run_snd_fst_of_le x (by omega)]
+    simp
+    rw [cond_eq_if, if_pos]; simp; omega
+  | .const b =>
+    simp [traceEval, traceEval.run, size] at *
+    rw [traceEval_run_snd_fst_of_le x (by omega)]
+    simp
+    rw [cond_eq_if, if_pos]; simp; omega
+  | .not y =>
+    have t : x.size - 1 + 1 = x.size := by omega
+    simp [traceEval, traceEval.run, size] at *
+    rw [traceEval_run_snd_fst_of_le x (by omega)]
+    simp
+    if h : l < x.size + y.size then
+      rw [traceEval_run_snd_fst y (by omega) (by omega),
+        traceEval_run_snd_fst y (by omega) (by omega)]
+      simp [t]
+    else
+      rw [traceEval_run_snd_fst_of_le y (by omega),
+        traceEval_run_snd_fst_of_le y (by omega)]
+      rw [cond_eq_if, if_pos]
+      · simp [t]
+      · simp; omega
+  | .gate g y z =>
+    have := y.size_pos
+    have := z.size_pos
+    have t : x.size - 1 + 1 = x.size := by omega
+    simp [traceEval, traceEval.run, size] at *
+    rw [traceEval_run_snd_fst_of_le x (by omega)]
+    if h : l < x.size + y.size then
+      rw [traceEval_run_snd_fst y (by omega) (by omega),
+        traceEval_run_snd_fst y (by omega) (by omega)]
+      simp [t]
+    else
+      if h : l < x.size + y.size + z.size then
+        rw [traceEval_run_snd_fst z (by omega) (by omega),
+          traceEval_run_snd_fst z (by omega) (by omega)]
+        simp [t]
+      else
+        rw [traceEval_run_snd_fst_of_le y (by omega), traceEval_run_snd_fst_of_le y (by omega), traceEval_run_snd_fst_of_le z (by omega),
+          traceEval_run_snd_fst_of_le z (by omega)]
+        simp [cond_eq_if]
+        rw [if_pos]
+        simp [t]
+        omega
+
+theorem eval_elim_traceEval_not (f : α → Bool) (x) :
+    CNF.eval (Sum.elim f (traceEval (not x) f)) (toCNF'.run 0 x).1 =
+      CNF.eval (Sum.elim f (traceEval x f)) (toCNF'.run 0 x).1 := by
+  apply CNF.eval_congr
+  rintro (a | i)
+  · simp
+  · simp
+    intro h
+    replace h := lt_of_inr_mem_toCNF'_run_fst h
+    simp at h
+    exact traceEval_not h
+
+theorem eval_elim_traceEval_gate_left (f : α → Bool) (g) (x) (y) :
+    CNF.eval (Sum.elim f (traceEval (gate g x y) f)) (toCNF'.run 0 x).1 =
+      CNF.eval (Sum.elim f (traceEval x f)) (toCNF'.run 0 x).1 := by
+  apply CNF.eval_congr
+  rintro (a | i)
+  · simp
+  · simp
+    intro h
+    replace h := lt_of_inr_mem_toCNF'_run_fst h
+    simp at h
+    exact traceEval_gate_left h
+
+theorem eval_elim_traceEval_gate_right (f : α → Bool) (g) (x) (y) :
+    CNF.eval (Sum.elim f (traceEval (gate g x y) f)) (toCNF'.run x.size y).1 =
+      CNF.eval (Sum.elim f (traceEval y f)) (toCNF'.run 0 y).1 := by
+  apply Eq.trans
+  apply CNF.eval_congr
+  rotate_left
+  exact Sum.elim f (fun l => (traceEval.run f l x.size y).1)
+  rotate_left
+  · rintro (a | i)
+    · simp_all
+    · simp only [Sum.elim_inr]
+      intro h
+      replace h := bounds_of_inr_mem_toCNF'_run_fst h
+      exact traceEval_gate_right h.1 h.2
+  · rw [toCNF'.run_fst_eq_relabel x.size y]
+    rw [elim_traceEval_eq_comp x.size]
+    apply CNF.eval_relabel
 
 theorem toCNF'_run_fst_eval_elim_traceEval (x : BoolExpr α) (f : α → Bool) :
     (toCNF'.run 0 x).1.eval (Sum.elim f (x.traceEval f)) = true := by
@@ -280,14 +525,31 @@ theorem toCNF'_run_fst_eval_elim_traceEval (x : BoolExpr α) (f : α → Bool) :
     have := x.size_pos
     have := toCNF'_run_fst_eval_elim_traceEval x f
     revert this
-    simp only [toCNF'.run, toCNF'_run_snd, Nat.zero_add, CNF.eval_append, CNF.ne_eval, Sum.elim_inr,
-      traceEval, traceEval.run, Nat.succ.injEq, Bool.and_eq_true, beq_iff_eq]
-    rw [traceEval_run_snd_fst_of_le, traceEval_run_snd_fst, traceEval_run_fst, traceEval_run_fst]
-    have : CNF.eval (Sum.elim f (traceEval (not x) f)) (toCNF'.run 0 x).fst = CNF.eval (Sum.elim f (traceEval x f)) (toCNF'.run 0 x).fst := sorry
+    simp [toCNF'.run, traceEval, traceEval.run]
+    rw [traceEval_run_snd_fst_of_le x (by omega), traceEval_run_snd_fst x (by omega) (by omega),
+      traceEval_run_fst (by omega), traceEval_run_fst (by omega)]
+    have := eval_elim_traceEval_not f x
     rw [this]
     simp only [cond_false, cond_true, true_and, imp_self]
-    all_goals omega
-  | .gate g x y => sorry
+  | .gate g x y =>
+    have := x.size_pos
+    have := y.size_pos
+    have t : x.size - 1 + 1 = x.size := by omega
+    have := toCNF'_run_fst_eval_elim_traceEval x f
+    revert this
+    have := toCNF'_run_fst_eval_elim_traceEval y f
+    revert this
+    simp [toCNF'.run, traceEval, traceEval.run, t]
+    have := eval_elim_traceEval_gate_left f g x y
+    rw [this]
+    have := eval_elim_traceEval_gate_right f g x y
+    rw [this]
+    rw [traceEval_run_snd_fst_of_le x (by omega), traceEval_run_snd_fst_of_le y (by omega),
+       traceEval_run_snd_fst x (by omega) (by omega),  traceEval_run_snd_fst_of_le x (by omega),
+      traceEval_run_fst (by omega), traceEval_run_fst (by omega), traceEval_run_fst (by omega)]
+    simp
+    rw [traceEval_run_snd_fst y (by omega) (by omega), traceEval_run_fst (by omega)]
+    simp_all
 
 theorem toCNF'_eval_elim_traceEval (x : BoolExpr α) (f : α → Bool) :
     (toCNF' x).eval (Sum.elim f (x.traceEval f)) = x.eval f := by
@@ -298,13 +560,23 @@ theorem toCNF'_eval_elim_traceEval (x : BoolExpr α) (f : α → Bool) :
     dsimp [toCNF']
     have := toCNF'_run_fst_eval_elim_traceEval x f
     revert this
-    simp [toCNF'.run]
-    have : CNF.eval (Sum.elim f (traceEval (not x) f)) (toCNF'.run 0 x).fst = CNF.eval (Sum.elim f (traceEval x f)) (toCNF'.run 0 x).fst := sorry
-    rw [this]
-    generalize CNF.eval (Sum.elim f (traceEval x f)) (toCNF'.run 0 x).fst = x1
-    cases x1 <;> simp
-    sorry
-  | .gate g x y => sorry
+    have := toCNF'_run_fst_eval_elim_traceEval (not x) f
+    revert this
+    generalize CNF.eval (Sum.elim f (traceEval x f)) _ = x1
+    generalize CNF.eval (Sum.elim f (traceEval (not x) f)) _ = x2
+    cases x1 <;> cases x2 <;> simp
+  | .gate g x y =>
+    dsimp [toCNF']
+    have := toCNF'_run_fst_eval_elim_traceEval x f
+    revert this
+    have := toCNF'_run_fst_eval_elim_traceEval y f
+    revert this
+    have := toCNF'_run_fst_eval_elim_traceEval (gate g x y) f
+    revert this
+    generalize CNF.eval (Sum.elim f (traceEval x f)) _ = x1
+    generalize CNF.eval (Sum.elim f (traceEval y f)) _ = x2
+    generalize CNF.eval (Sum.elim f (traceEval (gate g x y) f)) _ = x3
+    cases x1 <;> cases x2 <;> cases x3 <;> simp
 
 theorem toCNF'_unsat {x : BoolExpr α} : (toCNF' x).unsat ↔ x.unsat := by
   constructor
