LeanSAT/Reflect/CNF/Basic.lean
@@ -5,6 +5,8 @@ Authors: Scott Morrison
 -/
 import LeanSAT.Reflect.CNF.ForStd
 import Std.Data.Bool
+import Std.Tactic.Omega
+import Std.Tactic.SimpTrace
 
 set_option linter.missingDocs false
 
@@ -18,7 +20,7 @@ def Clause.eval (f : α → Bool) (c : Clause α) : Bool := c.any fun (i, n) => 
 
 @[simp] theorem Clause.eval_nil (f : α → Bool) : Clause.eval f [] = false := rfl
 @[simp] theorem Clause.eval_succ (f : α → Bool) :
-    Clause.eval f ((a, b) :: c) = ((xor b (f a)) || Clause.eval f c) := rfl
+    Clause.eval f (i :: c) = ((xor i.2 (f i.1)) || Clause.eval f c) := rfl
 
 def eval (f : α → Bool) (g : CNF α) : Bool := g.all fun c => c.eval f
 
@@ -31,4 +33,44 @@ def eval (f : α → Bool) (g : CNF α) : Bool := g.all fun c => c.eval f
 def sat (g : CNF α) (f : α → Bool) : Prop := eval f g = true
 def unsat (g : CNF α) : Prop := ∀ f, eval f g = false
 
-end CNF
+namespace Clause
+
+def mem (a : α) (c : Clause α) : Prop := (a, false) ∈ c ∨ (a, true) ∈ c
+
+instance : Membership α (Clause α) := ⟨mem⟩
+
+@[simp] theorem not_mem_nil {a : α} : a ∈ ([] : Clause α) ↔ False := sorry
+@[simp] theorem mem_cons {a : α} : (a ∈ (i :: c : Clause α)) ↔ (a = i.1 ∨ a ∈ c) := sorry
+
+theorem eval_congr (f g : α → Bool) (c : Clause α) (w : ∀ i, i ∈ c → f i = g i) :
+    eval f c = eval g c := by
+  induction c
+  case nil => rfl
+  case cons i c ih =>
+    simp only [eval_succ]
+    rw [ih, w]
+    · sorry
+    · intro j h
+      apply w
+      sorry
+
+end Clause
+
+def mem (a : α) (g : CNF α) : Prop := ∃ c, c ∈ g ∧ c.mem a
+
+instance : Membership α (CNF α) := ⟨mem⟩
+
+@[simp] theorem not_mem_nil {a : α} : a ∈ ([] : CNF α) ↔ False := sorry
+@[simp] theorem mem_cons {a : α} {i} {c : CNF α} : (a ∈ (i :: c : CNF α)) ↔ (a ∈ i ∨ a ∈ c) := sorry
+
+@[simp] theorem mem_append {a : α} {x y : CNF α} : a ∈ x ++ y ↔ a ∈ x ∨ a ∈ y := sorry
+
+theorem eval_congr (f g : α → Bool) (x : CNF α) (w : ∀ i, i ∈ x → f i = g i) :
+    eval f x = eval g x := by
+  induction x
+  case nil => rfl
+  case cons c x ih =>
+    simp only [eval_succ]
+    rw [ih, Clause.eval_congr]
+    · sorry
+    · sorry
