LeanSAT/Reflect/CNF/Relabel.lean
@@ -7,26 +7,74 @@ import LeanSAT.Reflect.CNF.Basic
 
 set_option linter.missingDocs false
 
+@[simp] theorem _root_.List.map_replicate :
+    (List.replicate n a).map f = List.replicate n (f a) := by
+  induction n <;> simp_all
+
 namespace CNF
 
 namespace Clause
 
 def relabel (f : α → β) (c : Clause α) : Clause β := c.map (fun (i, n) => (f i, n))
 
-def maxLiteral (c : Clause Nat) : Option Nat := (c.map (·.1)) |>.minimum?
+@[simp] theorem eval_relabel {f : α → β} {g : β → Bool} {x : Clause α} :
+    (relabel f x).eval g = x.eval (g ∘ f) := by
+  induction x <;> simp_all [relabel]
 
 end Clause
 
 /-! ### Relabelling
 
 It is convenient to be able to construct a CNF using a more complicated literal type,
-but eventually we need to embed in Nat.
+but eventually we need to embed in `Nat`.
 -/
 
 def relabel (f : α → β) (g : CNF α) : CNF β := g.map (Clause.relabel f)
 
-theorem sat_relabel (h : sat g (k ∘ f)) : sat (relabel k g) f := sorry
-theorem unsat_relabel (h : unsat g) : unsat (relabel k g) := sorry
-theorem unsat_relabel_iff (w : ∀ a b, k a = k b → a = b) : unsat (relabel k g) ↔ unsat g := sorry
+@[simp] theorem eval_relabel (f : α → β) (g : β → Bool) (x : CNF α) :
+    (relabel f x).eval g = x.eval (g ∘ f) := by
+  induction x <;> simp_all [relabel]
+
+theorem sat_relabel (h : sat x (g ∘ f)) : sat (relabel f x) g := by
+  simp_all [sat]
+
+theorem unsat_relabel {x : CNF α} (f : α → β) (h : unsat x) : unsat (relabel f x) := by
+  simp_all [unsat]
+
+theorem nonempty_or_impossible (x : CNF α) : Nonempty α ∨ ∃ n, x = List.replicate n [] := by
+  induction x with
+  | nil => exact Or.inr ⟨0, rfl⟩
+  | cons c x ih => match c with
+    | [] => cases ih with
+      | inl h => left; exact h
+      | inr h =>
+        obtain ⟨n, rfl⟩ := h
+        right
+        exact ⟨n + 1, rfl⟩
+    | ⟨a, b⟩ :: c => exact Or.inl ⟨a⟩
+
+theorem unsat_relabel_iff {x : CNF α} {f : α → β} (w : ∀ a b, f a = f b → a = b) :
+    unsat (relabel f x) ↔ unsat x := by
+  rcases nonempty_or_impossible x with (⟨⟨a₀⟩⟩ | ⟨n, rfl⟩)
+  · refine ⟨fun h => ?_, unsat_relabel f⟩
+    have em := Classical.propDecidable
+    let g : β → α := fun b =>
+      if h : ∃ a, f a = b then h.choose else a₀
+    have h' := unsat_relabel g h
+    suffices w : relabel g (relabel f x) = x by
+      rwa [w] at h'
+    simp only [relabel, List.map_map]
+    suffices w : Clause.relabel _ ∘ Clause.relabel _ = id by
+      rw [w, List.map_id]
+    funext c
+    simp only [Function.comp_apply, id_eq, Clause.relabel, List.map_map]
+    suffices w : _ ∘ _ = id by
+      rw [w, List.map_id]
+    funext ⟨a, b⟩
+    simp only [Function.comp_apply, exists_apply_eq_apply, ↓reduceDite, id_eq]
+    congr
+    apply w
+    exact Exists.choose_spec (⟨a, rfl⟩ : ∃ a', f a' = f a)
+  · cases n <;> simp [unsat, relabel, Clause.relabel]
 
 end CNF
